\documentclass[12pt]{article}
\usepackage{lingmacros}
\usepackage{tree-dvips}
\begin{document}

$\frac{dv}{dt} = -v + I$

$\rightarrow$ $\frac{v(t+\Delta t)-v(t)}{\Delta t} = -v(t)+I$ \\
$v(t+\Delta t)-v(t) = \Delta t(-v(t)+I) $ \\


$v(t+\Delta t) = v(t)+\Delta t(-v(t)+I)$ \\


we could say:\\
\begin{center}
			t = n$\Delta t$\\
\end{center}
Hence: \\
	\begin{center}
	v((n+1)$\Delta t$) = v(n$\Delta$t) + $\Delta$t(-v(n$\Delta$t)+I)\\
	\end{center}

For having a simpler formula:\\
	\begin{center}
		$v_{n+1} = v_n + \Delta t (-v_n+I)$\\
	\end{center}



\end{document}

